theories/RocqsheetCofix.v
@@ -1,9 +1,4 @@
 (* Copyright (c) 2026 CharlesCNorton.  Licensed under the MIT License. *)
-(* Coinductive evaluator for the Rocqsheet kernel.  Cycles are
-   caught by the visited-set check inside [trans], not by fuel.
-   Theorems use a bounded [run_n] driver so [vm_compute] can
-   discharge closed cases.  Not extracted. *)
-
 From Stdlib Require Import List BinInt.
 From Corelib Require Import PrimInt63.
 From Crane Require Import Mapping.NatIntStd Mapping.ZInt.
@@ -17,32 +12,43 @@ Open Scope int63.
 Definition NoE : Type -> Type := fun _ => Empty_set.
 
 Inductive Cont : Type :=
-  | KAddR  : list CellRef -> Expr -> Cont
-  | KAddL  : Z -> Cont
-  | KSubR  : list CellRef -> Expr -> Cont
-  | KSubL  : Z -> Cont
-  | KMulR  : list CellRef -> Expr -> Cont
-  | KMulL  : Z -> Cont
-  | KDivR  : list CellRef -> Expr -> Cont
-  | KDivL  : Z -> Cont
-  | KEqR   : list CellRef -> Expr -> Cont
-  | KEqL   : Z -> Cont
-  | KLtR   : list CellRef -> Expr -> Cont
-  | KLtL   : Z -> Cont
-  | KGtR   : list CellRef -> Expr -> Cont
-  | KGtL   : Z -> Cont
-  | KIf    : list CellRef -> Expr -> Expr -> Cont.
+  | KAddR    : list CellRef -> Expr -> Cont
+  | KAddL    : Z -> Cont
+  | KSubR    : list CellRef -> Expr -> Cont
+  | KSubL    : Z -> Cont
+  | KMulR    : list CellRef -> Expr -> Cont
+  | KMulL    : Z -> Cont
+  | KDivR    : list CellRef -> Expr -> Cont
+  | KDivL    : Z -> Cont
+  | KEqR     : list CellRef -> Expr -> Cont
+  | KEqL     : Z -> Cont
+  | KLtR     : list CellRef -> Expr -> Cont
+  | KLtL     : Z -> Cont
+  | KGtR     : list CellRef -> Expr -> Cont
+  | KGtL     : Z -> Cont
+  | KIf      : list CellRef -> Expr -> Expr -> Cont
+  | KModR    : list CellRef -> Expr -> Cont
+  | KModL    : Z -> Cont
+  | KPowR    : list CellRef -> Expr -> Cont
+  | KPowL    : Z -> Cont
+  | KNot     : Cont
+  | KAndR    : list CellRef -> Expr -> Cont
+  | KAndL    : Z -> Cont
+  | KOrR     : list CellRef -> Expr -> Cont
+  | KOrL     : Z -> Cont
+  | KSumNext : list CellRef -> int -> int -> int -> int -> int -> Z -> Cont
+  | KIfErr   : list CellRef -> Expr -> Cont.
 
 Inductive PC : Type :=
-  | PCEval  : list CellRef -> Expr -> PC
-  | PCApply : option Z -> PC.
+  | PCEval    : list CellRef -> Expr -> PC
+  | PCApply   : option Z -> PC
+  | PCSumStep : list CellRef -> int -> int -> int -> int -> int -> Z -> PC.
 
 Record State : Type := mkSt
   { st_sheet : Sheet
   ; st_pc    : PC
   ; st_stack : list Cont }.
 
-(* One transition: either a successor state or a terminal value. *)
 Definition trans (st : State) : State + option Z :=
   match st_pc st with
   | PCEval visited (EInt n) =>
@@ -54,6 +60,7 @@ Definition trans (st : State) : State + option Z :=
         match get_cell (st_sheet st) r with
         | CEmpty   => inl (mkSt (st_sheet st) (PCApply (Some 0%Z)) (st_stack st))
         | CLit n   => inl (mkSt (st_sheet st) (PCApply (Some n)) (st_stack st))
+        | CFloat _ => inr None  (* cofix evaluator covers Z only *)
         | CForm e' => inl (mkSt (st_sheet st)
                                 (PCEval (r :: visited) e') (st_stack st))
         end
@@ -81,18 +88,70 @@ Definition trans (st : State) : State + option Z :=
   | PCEval visited (EIf c t e) =>
       inl (mkSt (st_sheet st) (PCEval visited c)
                (KIf visited t e :: st_stack st))
-  (* The cofix machine pre-dates EMod/EPow/ENot/EAnd/EOr/ESum.
-     Cofix support for those constructors would mean new
-     continuations and (for ESum) a separate sum-walking sub-state.
-     They terminate the trampoline with [None] for now; the five
-     closed-term theorems below are all in the original
-     sub-language and remain provable. *)
-  | PCEval _ (EMod _ _) | PCEval _ (EPow _ _)
-  | PCEval _ (ENot _)   | PCEval _ (EAnd _ _)
-  | PCEval _ (EOr  _ _) | PCEval _ (ESum _ _) =>
+  | PCEval visited (EMod a b) =>
+      inl (mkSt (st_sheet st) (PCEval visited a)
+               (KModR visited b :: st_stack st))
+  | PCEval visited (EPow a b) =>
+      inl (mkSt (st_sheet st) (PCEval visited a)
+               (KPowR visited b :: st_stack st))
+  | PCEval visited (ENot a) =>
+      inl (mkSt (st_sheet st) (PCEval visited a)
+               (KNot :: st_stack st))
+  | PCEval visited (EAnd a b) =>
+      inl (mkSt (st_sheet st) (PCEval visited a)
+               (KAndR visited b :: st_stack st))
+  | PCEval visited (EOr a b) =>
+      inl (mkSt (st_sheet st) (PCEval visited a)
+               (KOrR visited b :: st_stack st))
+  | PCEval visited (ESum tl br) =>
+      let lc := cell_col_of tl in
+      let hc := cell_col_of br in
+      let lr := cell_row_of tl in
+      let hr := cell_row_of br in
+      inl (mkSt (st_sheet st)
+                (PCSumStep visited lc hc lc lr hr 0%Z)
+                (st_stack st))
+  | PCEval visited (EAvg _ _) =>
       inr None
+  | PCEval visited (ECount tl br) =>
+      let lc := cell_col_of tl in
+      let hc := cell_col_of br in
+      let lr := cell_row_of tl in
+      let hr := cell_row_of br in
+      if orb (PrimInt63.ltb hc lc) (PrimInt63.ltb hr lr) then
+        inl (mkSt (st_sheet st) (PCApply (Some 0%Z)) (st_stack st))
+      else
+        let cs := PrimInt63.add (PrimInt63.sub hc lc) 1 in
+        let rs := PrimInt63.add (PrimInt63.sub hr lr) 1 in
+        inl (mkSt (st_sheet st)
+                  (PCApply (Some (Uint63.to_Z (PrimInt63.mul cs rs))))
+                  (st_stack st))
+  | PCEval visited (EIfErr a fb) =>
+      inl (mkSt (st_sheet st) (PCEval visited a)
+               (KIfErr visited fb :: st_stack st))
+  | PCEval _ (EFloat _) => inr None
+  | PCEval _ (EFAdd _ _) => inr None
+  | PCEval _ (EFSub _ _) => inr None
+  | PCEval _ (EFMul _ _) => inr None
+  | PCEval _ (EFDiv _ _) => inr None
+  | PCSumStep visited lc hc col row hr acc =>
+      if PrimInt63.ltb hr row then
+        inl (mkSt (st_sheet st) (PCApply (Some acc)) (st_stack st))
+      else if PrimInt63.ltb hc col then
+        inl (mkSt (st_sheet st)
+                  (PCSumStep visited lc hc lc
+                             (PrimInt63.add row 1) hr acc)
+                  (st_stack st))
+      else
+        inl (mkSt (st_sheet st)
+                  (PCEval visited (ERef (mkRef col row)))
+                  (KSumNext visited lc hc col row hr acc :: st_stack st))
   | PCApply None =>
-      inr None
+      match st_stack st with
+      | KIfErr vp fb :: k' =>
+          inl (mkSt (st_sheet st) (PCEval vp fb) k')
+      | _ => inr None
+      end
   | PCApply (Some v) =>
       match st_stack st with
       | [] => inr (Some v)
@@ -111,7 +170,8 @@ Definition trans (st : State) : State + option Z :=
       | KDivR vp b :: k' =>
           inl (mkSt (st_sheet st) (PCEval vp b) (KDivL v :: k'))
       | KDivL vL :: k' =>
-          if Z.eqb v 0%Z then inr None
+          if Z.eqb v 0%Z then
+            inl (mkSt (st_sheet st) (PCApply None) k')
           else inl (mkSt (st_sheet st) (PCApply (Some (Z.div vL v))) k')
       | KEqR vp b :: k' =>
           inl (mkSt (st_sheet st) (PCEval vp b) (KEqL v :: k'))
@@ -133,10 +193,46 @@ Definition trans (st : State) : State + option Z :=
             inl (mkSt (st_sheet st) (PCEval vp e) k')
           else
             inl (mkSt (st_sheet st) (PCEval vp t) k')
+      | KModR vp b :: k' =>
+          inl (mkSt (st_sheet st) (PCEval vp b) (KModL v :: k'))
+      | KModL vL :: k' =>
+          if Z.eqb v 0%Z then
+            inl (mkSt (st_sheet st) (PCApply None) k')
+          else inl (mkSt (st_sheet st) (PCApply (Some (Z.modulo vL v))) k')
+      | KPowR vp b :: k' =>
+          inl (mkSt (st_sheet st) (PCEval vp b) (KPowL v :: k'))
+      | KPowL vL :: k' =>
+          if Z.ltb v 0%Z then
+            inl (mkSt (st_sheet st) (PCApply None) k')
+          else inl (mkSt (st_sheet st) (PCApply (Some (Z.pow vL v))) k')
+      | KNot :: k' =>
+          inl (mkSt (st_sheet st)
+                    (PCApply (Some (if Z.eqb v 0%Z then 1%Z else 0%Z))) k')
+      | KAndR vp b :: k' =>
+          inl (mkSt (st_sheet st) (PCEval vp b) (KAndL v :: k'))
+      | KAndL vL :: k' =>
+          inl (mkSt (st_sheet st)
+                    (PCApply (Some (if andb (negb (Z.eqb vL 0%Z))
+                                            (negb (Z.eqb v 0%Z))
+                                    then 1%Z else 0%Z))) k')
+      | KOrR vp b :: k' =>
+          inl (mkSt (st_sheet st) (PCEval vp b) (KOrL v :: k'))
+      | KOrL vL :: k' =>
+          inl (mkSt (st_sheet st)
+                    (PCApply (Some (if orb (negb (Z.eqb vL 0%Z))
+                                           (negb (Z.eqb v 0%Z))
+                                    then 1%Z else 0%Z))) k')
+      | KSumNext visited lc hc col row hr acc :: k' =>
+          inl (mkSt (st_sheet st)
+                    (PCSumStep visited lc hc
+                               (PrimInt63.add col 1) row hr
+                               (Z.add acc v))
+                    k')
+      | KIfErr _ _ :: k' =>
+          inl (mkSt (st_sheet st) (PCApply (Some v)) k')
       end
   end.
 
-(* The recursive call sits directly under [Tau] for guardedness. *)
 CoFixpoint step (st : State) : itree NoE (option Z) :=
   match trans st with
   | inl st' => Tau (step st')
@@ -149,13 +245,12 @@ Definition eval_co (visited : list CellRef) (s : Sheet) (e : Expr)
 
 Definition eval_cell_co (s : Sheet) (r : CellRef) : itree NoE (option Z) :=
   match get_cell s r with
-  | CEmpty => Ret (Some 0%Z)
-  | CLit n => Ret (Some n)
-  | CForm e => eval_co (r :: nil) s e
+  | CEmpty   => Ret (Some 0%Z)
+  | CLit n   => Ret (Some n)
+  | CFloat _ => Ret None  (* cofix evaluator covers Z only *)
+  | CForm e  => eval_co (r :: nil) s e
   end.
 
-(* Bounded driver: takes up to [n] Tau steps.  [Vis] is unreachable
-   because [NoE] is empty. *)
 Fixpoint run_n (n : nat) (t : itree NoE (option Z)) : option (option Z) :=
   match n with
   | O => None
@@ -166,8 +261,6 @@ Fixpoint run_n (n : nat) (t : itree NoE (option Z)) : option (option Z) :=
     | _ => None
     end
   end.
-
-(* --- Closed-term theorems --- *)
 
 Theorem co_smoke :
   let a1 := mkRef 0 0 in
@@ -206,4 +299,124 @@ Theorem co_if_else :
   let s := set_cell new_sheet r
     (CForm (EIf (EInt 0%Z) (EInt 7%Z) (EInt 99%Z))) in
   run_n 50 (eval_cell_co s r) = Some (Some 99%Z).
+Proof. vm_compute. reflexivity. Qed.
+
+Theorem co_mod_smoke :
+  let r := mkRef 0 0 in
+  let s := set_cell new_sheet r
+    (CForm (EMod (EInt 10%Z) (EInt 3%Z))) in
+  run_n 50 (eval_cell_co s r) = Some (Some 1%Z).
+Proof. vm_compute. reflexivity. Qed.
+
+Theorem co_mod_zero :
+  let r := mkRef 0 0 in
+  let s := set_cell new_sheet r
+    (CForm (EMod (EInt 5%Z) (EInt 0%Z))) in
+  run_n 50 (eval_cell_co s r) = Some None.
+Proof. vm_compute. reflexivity. Qed.
+
+Theorem co_pow_smoke :
+  let r := mkRef 0 0 in
+  let s := set_cell new_sheet r
+    (CForm (EPow (EInt 2%Z) (EInt 10%Z))) in
+  run_n 50 (eval_cell_co s r) = Some (Some 1024%Z).
+Proof. vm_compute. reflexivity. Qed.
+
+Theorem co_pow_neg :
+  let r := mkRef 0 0 in
+  let s := set_cell new_sheet r
+    (CForm (EPow (EInt 2%Z) (EInt (-1)%Z))) in
+  run_n 50 (eval_cell_co s r) = Some None.
+Proof. vm_compute. reflexivity. Qed.
+
+Theorem co_not_zero :
+  let r := mkRef 0 0 in
+  let s := set_cell new_sheet r
+    (CForm (ENot (EInt 0%Z))) in
+  run_n 50 (eval_cell_co s r) = Some (Some 1%Z).
+Proof. vm_compute. reflexivity. Qed.
+
+Theorem co_not_nonzero :
+  let r := mkRef 0 0 in
+  let s := set_cell new_sheet r
+    (CForm (ENot (EInt 5%Z))) in
+  run_n 50 (eval_cell_co s r) = Some (Some 0%Z).
+Proof. vm_compute. reflexivity. Qed.
+
+Theorem co_and_true :
+  let r := mkRef 0 0 in
+  let s := set_cell new_sheet r
+    (CForm (EAnd (EInt 1%Z) (EInt 2%Z))) in
+  run_n 50 (eval_cell_co s r) = Some (Some 1%Z).
+Proof. vm_compute. reflexivity. Qed.
+
+Theorem co_and_false :
+  let r := mkRef 0 0 in
+  let s := set_cell new_sheet r
+    (CForm (EAnd (EInt 0%Z) (EInt 1%Z))) in
+  run_n 50 (eval_cell_co s r) = Some (Some 0%Z).
+Proof. vm_compute. reflexivity. Qed.
+
+Theorem co_or_true :
+  let r := mkRef 0 0 in
+  let s := set_cell new_sheet r
+    (CForm (EOr (EInt 0%Z) (EInt 1%Z))) in
+  run_n 50 (eval_cell_co s r) = Some (Some 1%Z).
+Proof. vm_compute. reflexivity. Qed.
+
+Theorem co_or_false :
+  let r := mkRef 0 0 in
+  let s := set_cell new_sheet r
+    (CForm (EOr (EInt 0%Z) (EInt 0%Z))) in
+  run_n 50 (eval_cell_co s r) = Some (Some 0%Z).
+Proof. vm_compute. reflexivity. Qed.
+
+Theorem co_sum_row :
+  let s := set_cell new_sheet (mkRef 0 0) (CLit 1%Z) in
+  let s := set_cell s (mkRef 1 0) (CLit 2%Z) in
+  let s := set_cell s (mkRef 2 0) (CLit 3%Z) in
+  let dst := mkRef 0 5 in
+  let s := set_cell s dst (CForm (ESum (mkRef 0 0) (mkRef 2 0))) in
+  run_n 200 (eval_cell_co s dst) = Some (Some 6%Z).
+Proof. vm_compute. reflexivity. Qed.
+
+Theorem co_sum_rect :
+  let s := set_cell new_sheet (mkRef 0 0) (CLit 1%Z) in
+  let s := set_cell s (mkRef 1 0) (CLit 2%Z) in
+  let s := set_cell s (mkRef 0 1) (CLit 3%Z) in
+  let s := set_cell s (mkRef 1 1) (CLit 4%Z) in
+  let dst := mkRef 0 5 in
+  let s := set_cell s dst (CForm (ESum (mkRef 0 0) (mkRef 1 1))) in
+  run_n 300 (eval_cell_co s dst) = Some (Some 10%Z).
+Proof. vm_compute. reflexivity. Qed.
+
+Theorem co_sum_singleton :
+  let r := mkRef 4 4 in
+  let dst := mkRef 0 5 in
+  let s := set_cell new_sheet r (CLit 42%Z) in
+  let s := set_cell s dst (CForm (ESum r r)) in
+  run_n 100 (eval_cell_co s dst) = Some (Some 42%Z).
+Proof. vm_compute. reflexivity. Qed.
+
+Theorem co_iferror_some_eq_first :
+  let r := mkRef 0 0 in
+  let s := set_cell new_sheet r
+    (CForm (EIfErr (EInt 42%Z) (EInt 99%Z))) in
+  run_n 50 (eval_cell_co s r) = Some (Some 42%Z).
+Proof. vm_compute. reflexivity. Qed.
+
+Theorem co_iferror_traps_divzero :
+  let r := mkRef 0 0 in
+  let s := set_cell new_sheet r
+    (CForm (EIfErr (EDiv (EInt 1%Z) (EInt 0%Z)) (EInt 99%Z))) in
+  run_n 50 (eval_cell_co s r) = Some (Some 99%Z).
+Proof. vm_compute. reflexivity. Qed.
+
+Theorem co_iferror_traps_cycle :
+  let r0 := mkRef 0 0 in
+  let r1 := mkRef 1 0 in
+  let s := set_cell new_sheet r0 (CForm (ERef r0)) in
+  let s := set_cell s r1
+    (CForm (EIfErr (ERef r0) (EInt 7%Z))) in
+  run_n 50 (eval_cell_co s r1) = Some (Some 7%Z).
 Proof. vm_compute. reflexivity. Qed.
