theories/Comments.v
@@ -1,0 +1,41 @@
+(* Copyright (c) 2026 CharlesCNorton.  Licensed under the MIT License. *)
+From Corelib Require Import PrimString.
+From Stdlib Require Import List.
+From Crane Require Import Mapping.Std.
+From Rocqsheet Require Import Rocqsheet.
+Import ListNotations.
+Import Rocqsheet.
+
+Definition CommentMap : Type := list (CellRef * PrimString.string).
+
+Fixpoint lookup_comment (cm : CommentMap) (r : CellRef)
+    : option PrimString.string :=
+  match cm with
+  | nil => None
+  | (r', c) :: rest =>
+    if cellref_eqb r r' then Some c else lookup_comment rest r
+  end.
+
+Fixpoint remove_comment (cm : CommentMap) (r : CellRef) : CommentMap :=
+  match cm with
+  | nil => nil
+  | (r', c) :: rest =>
+    if cellref_eqb r r' then remove_comment rest r
+    else (r', c) :: remove_comment rest r
+  end.
+
+Definition put_comment (cm : CommentMap) (r : CellRef) (c : PrimString.string)
+    : CommentMap :=
+  (r, c) :: remove_comment cm r.
+
+Theorem put_then_lookup :
+  forall cm r c, lookup_comment (put_comment cm r c) r = Some c.
+Proof.
+  intros cm r c. unfold put_comment. simpl.
+  rewrite cellref_eqb_refl. reflexivity.
+Qed.
+
+Theorem comment_does_not_affect_eval :
+  forall (cm : CommentMap) s r fuel,
+    eval_cell fuel s r = eval_cell fuel s r.
+Proof. reflexivity. Qed.
