theories/Date.v
@@ -1,0 +1,36 @@
+(* Copyright (c) 2026 CharlesCNorton.  Licensed under the MIT License. *)
+From Stdlib Require Import BinInt Lia.
+
+Open Scope Z_scope.
+
+Definition Date : Type := Z.
+
+Definition add_days (d : Date) (n : Z) : Date := d + n.
+
+Definition sub_days (d1 d2 : Date) : Z := d1 - d2.
+
+Definition weekday (d : Date) : Z := d mod 7.
+
+Theorem add_days_zero : forall d, add_days d 0 = d.
+Proof. intros. unfold add_days. lia. Qed.
+
+Theorem sub_days_self : forall d, sub_days d d = 0.
+Proof. intros. unfold sub_days. lia. Qed.
+
+Theorem weekday_add_seven : forall d,
+  weekday (add_days d 7) = weekday d.
+Proof.
+  intros. unfold weekday, add_days.
+  rewrite Z.add_mod by lia.
+  replace (7 mod 7) with 0 by reflexivity.
+  rewrite Z.add_0_r.
+  rewrite Z.mod_mod by lia.
+  reflexivity.
+Qed.
+
+Theorem add_days_no_overflow_in_range :
+  forall d n,
+    -1000000 <= d <= 1000000 ->
+    -1000000 <= n <= 1000000 ->
+    -2000000 <= add_days d n <= 2000000.
+Proof. intros. unfold add_days. lia. Qed.
