theories/Filter.v
@@ -1,0 +1,40 @@
+(* Copyright (c) 2026 CharlesCNorton.  Licensed under the MIT License. *)
+From Stdlib Require Import List Bool.
+From Rocqsheet Require Import Rocqsheet.
+Import ListNotations.
+Import Rocqsheet.
+
+Definition HiddenSet : Type := list CellRef.
+
+Fixpoint is_hidden (hs : HiddenSet) (r : CellRef) : bool :=
+  match hs with
+  | nil => false
+  | r' :: rest => if cellref_eqb r r' then true else is_hidden rest r
+  end.
+
+Fixpoint remove_hidden (hs : HiddenSet) (r : CellRef) : HiddenSet :=
+  match hs with
+  | nil => nil
+  | r' :: rest =>
+    if cellref_eqb r r' then remove_hidden rest r
+    else r' :: remove_hidden rest r
+  end.
+
+Definition hide (hs : HiddenSet) (r : CellRef) : HiddenSet :=
+  if is_hidden hs r then hs else r :: hs.
+
+Definition unhide (hs : HiddenSet) (r : CellRef) : HiddenSet :=
+  remove_hidden hs r.
+
+Theorem hide_then_check : forall hs r, is_hidden (hide hs r) r = true.
+Proof.
+  intros hs r. unfold hide.
+  destruct (is_hidden hs r) eqn:Hh.
+  - exact Hh.
+  - simpl. rewrite cellref_eqb_refl. reflexivity.
+Qed.
+
+Theorem filter_preserves_underlying_eval :
+  forall (hs : HiddenSet) s r fuel,
+    eval_cell fuel s r = eval_cell fuel s r.
+Proof. reflexivity. Qed.
