theories/FindReplace.v
@@ -1,0 +1,54 @@
+(* Copyright (c) 2026 CharlesCNorton.  Licensed under the MIT License. *)
+From Stdlib Require Import List BinInt.
+From Crane Require Import Mapping.NatIntStd Mapping.ZInt.
+From Rocqsheet Require Import Rocqsheet.
+Import ListNotations.
+Import Rocqsheet.
+
+Fixpoint replace_int_in_expr (from to : Z) (e : Expr) : Expr :=
+  match e with
+  | EInt n => if Z.eqb n from then EInt to else EInt n
+  | ERef r => ERef r
+  | EAdd a b => EAdd (replace_int_in_expr from to a) (replace_int_in_expr from to b)
+  | ESub a b => ESub (replace_int_in_expr from to a) (replace_int_in_expr from to b)
+  | EMul a b => EMul (replace_int_in_expr from to a) (replace_int_in_expr from to b)
+  | EDiv a b => EDiv (replace_int_in_expr from to a) (replace_int_in_expr from to b)
+  | EEq a b => EEq (replace_int_in_expr from to a) (replace_int_in_expr from to b)
+  | ELt a b => ELt (replace_int_in_expr from to a) (replace_int_in_expr from to b)
+  | EGt a b => EGt (replace_int_in_expr from to a) (replace_int_in_expr from to b)
+  | EIf c t f => EIf (replace_int_in_expr from to c)
+                     (replace_int_in_expr from to t)
+                     (replace_int_in_expr from to f)
+  | EMod a b => EMod (replace_int_in_expr from to a) (replace_int_in_expr from to b)
+  | EPow a b => EPow (replace_int_in_expr from to a) (replace_int_in_expr from to b)
+  | ENot a => ENot (replace_int_in_expr from to a)
+  | EAnd a b => EAnd (replace_int_in_expr from to a) (replace_int_in_expr from to b)
+  | EOr a b => EOr (replace_int_in_expr from to a) (replace_int_in_expr from to b)
+  | ESum tl br => ESum tl br
+  | EAvg tl br => EAvg tl br
+  | ECount tl br => ECount tl br
+  | EIfErr a fb => EIfErr (replace_int_in_expr from to a) (replace_int_in_expr from to fb)
+  | EFloat f => EFloat f
+  | EFAdd a b => EFAdd (replace_int_in_expr from to a) (replace_int_in_expr from to b)
+  | EFSub a b => EFSub (replace_int_in_expr from to a) (replace_int_in_expr from to b)
+  | EFMul a b => EFMul (replace_int_in_expr from to a) (replace_int_in_expr from to b)
+  | EFDiv a b => EFDiv (replace_int_in_expr from to a) (replace_int_in_expr from to b)
+  end.
+
+Theorem replace_idempotent_when_equal :
+  forall n e, replace_int_in_expr n n e = e.
+Proof.
+  intros n e. induction e; simpl; try reflexivity;
+    try (rewrite IHe1; rewrite IHe2; reflexivity);
+    try (rewrite IHe; reflexivity).
+  - destruct (Z.eqb z n) eqn:H.
+    + apply Z.eqb_eq in H. subst. reflexivity.
+    + reflexivity.
+  - rewrite IHe1, IHe2, IHe3. reflexivity.
+Qed.
+
+Theorem replace_int_smoke :
+  let e := EAdd (EInt 1%Z) (EMul (EInt 2%Z) (EInt 1%Z)) in
+  replace_int_in_expr 1%Z 99%Z e =
+    EAdd (EInt 99%Z) (EMul (EInt 2%Z) (EInt 99%Z)).
+Proof. vm_compute. reflexivity. Qed.
