theories/NamedRanges.v
@@ -1,0 +1,53 @@
+(* Copyright (c) 2026 CharlesCNorton.  Licensed under the MIT License. *)
+From Corelib Require Import PrimString PrimInt63.
+From Stdlib Require Import List.
+From Crane Require Import Mapping.Std.
+From Rocqsheet Require Import Rocqsheet.
+Import ListNotations.
+Import Rocqsheet.
+
+Definition NameMap : Type := list (PrimString.string * CellRef).
+
+Definition pstring_eqb (a b : PrimString.string) : bool :=
+  match PrimString.compare a b with
+  | Eq => true
+  | _ => false
+  end.
+
+Fixpoint lookup_name (nm : NameMap) (n : PrimString.string)
+    : option CellRef :=
+  match nm with
+  | nil => None
+  | (n', r) :: rest =>
+    if pstring_eqb n n' then Some r else lookup_name rest n
+  end.
+
+Fixpoint remove_name (nm : NameMap) (n : PrimString.string) : NameMap :=
+  match nm with
+  | nil => nil
+  | (n', r) :: rest =>
+    if pstring_eqb n n' then remove_name rest n
+    else (n', r) :: remove_name rest n
+  end.
+
+Definition define_name (nm : NameMap) (n : PrimString.string) (r : CellRef)
+    : NameMap :=
+  (n, r) :: remove_name nm n.
+
+Theorem lookup_after_define_smoke :
+  let nm : NameMap := nil in
+  let nm' := define_name nm "myCell" (mkRef 3 5) in
+  lookup_name nm' "myCell" = Some (mkRef 3 5).
+Proof. vm_compute. reflexivity. Qed.
+
+Theorem lookup_undefined_smoke :
+  let nm : NameMap := nil in
+  lookup_name nm "missing" = None.
+Proof. reflexivity. Qed.
+
+Theorem define_then_undefine_smoke :
+  let nm : NameMap := nil in
+  let nm' := define_name nm "x" (mkRef 0 0) in
+  let nm'' := remove_name nm' "x" in
+  lookup_name nm'' "x" = None.
+Proof. vm_compute. reflexivity. Qed.
