theories/Saturation.v
@@ -1,0 +1,108 @@
+(* Copyright (c) 2026 CharlesCNorton.  Licensed under the MIT License. *)
+From Stdlib Require Import BinInt Lia Bool.
+
+Open Scope Z_scope.
+
+Definition INT64_MIN : Z := -9223372036854775808.
+Definition INT64_MAX : Z :=  9223372036854775807.
+
+Definition sat_add (a b : Z) : Z :=
+  let r := a + b in
+  if Z.ltb r INT64_MIN then INT64_MIN
+  else if Z.ltb INT64_MAX r then INT64_MAX
+  else r.
+
+Definition sat_sub (a b : Z) : Z :=
+  let r := a - b in
+  if Z.ltb r INT64_MIN then INT64_MIN
+  else if Z.ltb INT64_MAX r then INT64_MAX
+  else r.
+
+Definition sat_mul (a b : Z) : Z :=
+  let r := a * b in
+  if Z.ltb r INT64_MIN then INT64_MIN
+  else if Z.ltb INT64_MAX r then INT64_MAX
+  else r.
+
+Definition div_guard (a b : Z) : Z :=
+  if Z.eqb b 0 then 0
+  else if Z.eqb a INT64_MIN && Z.eqb b (-1) then INT64_MIN
+  else Z.div a b.
+
+Definition mod_guard (a b : Z) : Z :=
+  if Z.eqb b 0 then 0
+  else if Z.eqb a INT64_MIN && Z.eqb b (-1) then 0
+  else Z.modulo a b.
+
+Theorem sat_add_correct : forall a b,
+  (INT64_MIN <= a + b <= INT64_MAX -> sat_add a b = a + b) /\
+  (a + b > INT64_MAX -> sat_add a b = INT64_MAX) /\
+  (a + b < INT64_MIN -> sat_add a b = INT64_MIN).
+Proof.
+  intros a b. unfold sat_add.
+  destruct (Z.ltb (a+b) INT64_MIN) eqn:H1.
+  - apply Z.ltb_lt in H1.
+    repeat split; intros; unfold INT64_MIN, INT64_MAX in *; lia.
+  - apply Z.ltb_ge in H1.
+    destruct (Z.ltb INT64_MAX (a+b)) eqn:H2.
+    + apply Z.ltb_lt in H2.
+      repeat split; intros; unfold INT64_MIN, INT64_MAX in *; lia.
+    + apply Z.ltb_ge in H2.
+      repeat split; intros; unfold INT64_MIN, INT64_MAX in *; lia.
+Qed.
+
+Theorem sat_sub_correct : forall a b,
+  (INT64_MIN <= a - b <= INT64_MAX -> sat_sub a b = a - b) /\
+  (a - b > INT64_MAX -> sat_sub a b = INT64_MAX) /\
+  (a - b < INT64_MIN -> sat_sub a b = INT64_MIN).
+Proof.
+  intros a b. unfold sat_sub.
+  destruct (Z.ltb (a-b) INT64_MIN) eqn:H1.
+  - apply Z.ltb_lt in H1. repeat split; intros; unfold INT64_MIN, INT64_MAX in *; lia.
+  - apply Z.ltb_ge in H1.
+    destruct (Z.ltb INT64_MAX (a-b)) eqn:H2.
+    + apply Z.ltb_lt in H2. repeat split; intros; unfold INT64_MIN, INT64_MAX in *; lia.
+    + apply Z.ltb_ge in H2. repeat split; intros; unfold INT64_MIN, INT64_MAX in *; lia.
+Qed.
+
+Theorem sat_mul_correct : forall a b,
+  (INT64_MIN <= a * b <= INT64_MAX -> sat_mul a b = a * b) /\
+  (a * b > INT64_MAX -> sat_mul a b = INT64_MAX) /\
+  (a * b < INT64_MIN -> sat_mul a b = INT64_MIN).
+Proof.
+  intros a b. unfold sat_mul.
+  destruct (Z.ltb (a*b) INT64_MIN) eqn:H1.
+  - apply Z.ltb_lt in H1. repeat split; intros; unfold INT64_MIN, INT64_MAX in *; lia.
+  - apply Z.ltb_ge in H1.
+    destruct (Z.ltb INT64_MAX (a*b)) eqn:H2.
+    + apply Z.ltb_lt in H2. repeat split; intros; unfold INT64_MIN, INT64_MAX in *; lia.
+    + apply Z.ltb_ge in H2. repeat split; intros; unfold INT64_MIN, INT64_MAX in *; lia.
+Qed.
+
+Theorem div_guard_zero : forall a, div_guard a 0 = 0.
+Proof. intros. unfold div_guard. reflexivity. Qed.
+
+Theorem div_guard_int_min : div_guard INT64_MIN (-1) = INT64_MIN.
+Proof. unfold div_guard. reflexivity. Qed.
+
+Theorem div_guard_normal : forall a b,
+  b <> 0 ->
+  ~(a = INT64_MIN /\ b = -1) ->
+  div_guard a b = Z.div a b.
+Proof.
+  intros a b Hne Hno_min.
+  unfold div_guard.
+  destruct (Z.eqb b 0) eqn:H1.
+  - apply Z.eqb_eq in H1. contradiction.
+  - destruct (Z.eqb a INT64_MIN && Z.eqb b (-1)) eqn:H2.
+    + apply andb_prop in H2 as [H2a H2b].
+      apply Z.eqb_eq in H2a, H2b.
+      exfalso. apply Hno_min. split; assumption.
+    + reflexivity.
+Qed.
+
+Theorem mod_guard_zero : forall a, mod_guard a 0 = 0.
+Proof. intros. unfold mod_guard. reflexivity. Qed.
+
+Theorem mod_guard_int_min : mod_guard INT64_MIN (-1) = 0.
+Proof. unfold mod_guard. reflexivity. Qed.
